Proof for state_map order

Uppaal_Networks/UPPAAL_Asm_AbsInt.thy
@@ -4,12 +4,85 @@ imports
   "HOL.List"
 begin
 
-type_synonym 'a astate = "addr \<rightharpoonup> 'a"
+subsection "State Map"
+
+datatype 'a state_map = SM "addr \<rightharpoonup> 'a"
+fun lookup :: "'a state_map \<Rightarrow> addr \<Rightarrow> 'a option" where "lookup (SM m) = m"
+fun domain :: "'a state_map \<Rightarrow> addr set" where "domain (SM m) = dom m"
+
+lemma state_map_eq_fwd: "(\<forall>p. lookup m p = lookup n p) \<Longrightarrow> m = n"
+proof -
+  assume lookeq: "\<forall>p. lookup m p = lookup n p"
+  obtain mm where mm: "m = SM mm" using lookup.cases by blast
+  obtain nm where nm: "n = SM nm" using lookup.cases by blast
+  have "mm = nm" using lookeq nm mm by auto
+  thus "m = n" using mm nm by blast
+qed
+
+lemma "(\<forall>p. lookup m p = lookup n p) \<longleftrightarrow> m = n" using state_map_eq_fwd by auto
+
+(* -- *)
+(* From HOL_IMP.Abs_Int0 *)
+instantiation option :: (order)order
+begin
+
+fun less_eq_option where
+"Some x \<le> Some y = (x \<le> y)" |
+"None \<le> y = True" |
+"Some _ \<le> None = False"
+
+definition less_option where "x < (y::'a option) = (x \<le> y \<and> \<not> y \<le> x)"
+
+lemma le_None[simp]: "(x \<le> None) = (x = None)"
+by (cases x) simp_all
+
+lemma Some_le[simp]: "(Some x \<le> u) = (\<exists>y. u = Some y \<and> x \<le> y)"
+by (cases u) auto
+
+instance
+proof (standard, goal_cases)
+  case 1 show ?case by(rule less_option_def)
+next
+  case (2 x) show ?case by(cases x, simp_all)
+next
+  case (3 x y z) thus ?case by(cases z, simp, cases y, simp, cases x, auto)
+next
+  case (4 x y) thus ?case by(cases y, simp, cases x, auto)
+qed
+
+end
+(* -- *)
+
+instantiation state_map :: (order) order
+begin
+
+definition less_eq_state_map :: "('a::order)state_map \<Rightarrow> 'a state_map \<Rightarrow> bool" where
+"C1 \<le> C2 \<longleftrightarrow> (\<forall>p. lookup C1 p \<le> lookup C2 p)"
+
+definition less_state_map :: "'a state_map \<Rightarrow> 'a state_map \<Rightarrow> bool" where
+"less_state_map x y = (x \<le> y \<and> \<not> y \<le> x)"
+
+instance
+proof (standard, goal_cases)
+  case 1 show ?case by(simp add: less_state_map_def)
+next
+  case 2 thus ?case by(auto simp: less_eq_state_map_def)
+next
+  case 3 thus ?case using less_eq_state_map_def order_trans by fastforce
+next
+  case 4 thus ?case by (simp add: less_eq_state_map_def dual_order.antisym state_map_eq_fwd)
+qed
+
+end
+
+
+subsection "Collecting Semantics"
+
 type_synonym cpstate = "stack * rstate * flag * nat list"
-type_synonym collect_ctx = "(cpstate set astate) * (addr set)"
+type_synonym collect_ctx = "(cpstate set state_map) * (addr set)"
 
 fun collect_ctx_dom :: "collect_ctx \<Rightarrow> addr set" where "collect_ctx_dom (_, d) = d"
-fun collect_ctx_lookup :: "collect_ctx \<Rightarrow> addr \<Rightarrow> cpstate set option" where "collect_ctx_lookup (m, _) k = m k"
+fun collect_ctx_lookup :: "collect_ctx \<Rightarrow> addr \<Rightarrow> cpstate set option" where "collect_ctx_lookup (SM m, _) k = m k"
 
 fun def :: "'a \<Rightarrow> 'a option \<Rightarrow> 'a" where
   "def _ (Some v) = v" |
@@ -22,14 +95,14 @@ fun states_at :: "state set \<Rightarrow> addr \<Rightarrow> cpstate set" where
   "states_at states pc = snd ` {s\<in>states. fst s = pc}"
 
 fun propagate :: "collect_ctx \<Rightarrow> state set \<Rightarrow> collect_ctx" where
-  "propagate (oldst, olddom) ss =
+  "propagate (SM oldmap, olddom) ss =
     (let newdom = olddom \<union> states_domain ss;
          newmap = (\<lambda>pc.
             let news = states_at ss pc in
-            case (oldst pc, news) of
+            case (oldmap pc, news) of
               (Some oldss, newss) \<Rightarrow> Some (oldss \<union> news) |
               (None, newss) \<Rightarrow> if newss = {} then None else Some newss)
-    in (newmap, newdom))"
+    in (SM newmap, newdom))"
 
 fun step_all :: "instr \<Rightarrow> addr \<Rightarrow> cpstate set \<Rightarrow> state set" where
   "step_all op pc instates =
